Strata/DL/Imperative/KleeneStmt.lean
@@ -1,0 +1,112 @@
+/-
+  Copyright Strata Contributors
+
+  SPDX-License-Identifier: Apache-2.0 OR MIT
+-/
+module
+
+public import Strata.DL.Imperative.MetaData
+public import Strata.DL.Imperative.Stmt
+public import Strata.DL.Imperative.HasVars
+
+---------------------------------------------------------------------
+
+namespace Imperative
+
+public section
+
+/-! # Imperative dialect: Kleene statements
+
+These statements use assumptions to encode conditional branches and guarded
+loops. This is roughly the structure used by most formalizations of [Guarded
+Commands](https://en.wikipedia.org/wiki/Guarded_Command_Language), and in
+[Kleene Algebra with Tests](https://www.cs.cornell.edu/~kozen/Papers/kat.pdf).
+-/
+
+/--
+A Kleene statement, parameterized by a type of pure expressions (`P`)
+and a type of commands (`Cmd`).
+
+This encodes the same types of control flow as `Stmt`, but using only
+non-deterministic choices: arbitrarily choosing one of two sub-statements to
+execute or executing a sub-statement an arbitrary number of times. Conditions
+can be encoded if the command type includes assumptions.
+-/
+inductive KleeneStmt (P : PureExpr) (Cmd : Type) : Type where
+  /-- An atomic command, of an arbitrary type. -/
+  | cmd      (cmd : Cmd)
+  /-- Execute `s1` followed by `s2`. -/
+  | seq      (s1 s2 : KleeneStmt P Cmd)
+  /-- Execute either `s1` or `s2`, arbitrarily. -/
+  | choice   (s1 s2 : KleeneStmt P Cmd)
+  /-- Execute `s` an arbitrary number of times (possibly zero). -/
+  | loop     (s : KleeneStmt P Cmd)
+  deriving Inhabited
+
+abbrev KleeneStmt.init {P : PureExpr} (name : P.Ident) (ty : P.Ty) (expr : P.Expr) (md : MetaData P) :=
+  KleeneStmt.cmd (P:=P) (Cmd.init name ty (.det expr) md)
+abbrev KleeneStmt.set {P : PureExpr} (name : P.Ident) (expr : P.Expr) (md : MetaData P) :=
+  KleeneStmt.cmd (P:=P) (Cmd.set name (.det expr) md)
+abbrev KleeneStmt.havoc {P : PureExpr} (name : P.Ident) (md : MetaData P) :=
+  KleeneStmt.cmd (P:=P) (Cmd.set name .nondet md)
+abbrev KleeneStmt.assert {P : PureExpr} (label : String) (b : P.Expr) (md : MetaData P) :=
+  KleeneStmt.cmd (P:=P) (Cmd.assert label b md)
+abbrev KleeneStmt.assume {P : PureExpr} (label : String) (b : P.Expr) (md : MetaData P) :=
+  KleeneStmt.cmd (P:=P) (Cmd.assume label b md)
+
+mutual
+/-- Get all variables defined by the statement `s`. -/
+def KleeneStmt.definedVars [HasVarsImp P C] (s : KleeneStmt P C) : List P.Ident :=
+  match s with
+  | .cmd c => HasVarsImp.definedVars c
+  | .seq s1 s2 => KleeneStmt.definedVars s1 ++ KleeneStmt.definedVars s2
+  | .choice s1 s2 => KleeneStmt.definedVars s1 ++ KleeneStmt.definedVars s2
+  | .loop s => KleeneStmt.definedVars s
+
+def KleeneStmts.definedVars [HasVarsImp P C] (ss : List (KleeneStmt P C)) : List P.Ident :=
+  match ss with
+  | [] => []
+  | s :: srest => KleeneStmt.definedVars s ++ KleeneStmts.definedVars srest
+end
+
+mutual
+/-- Get all variables modified by the statement `s`. -/
+def KleeneStmt.modifiedVars [HasVarsImp P C] (s : KleeneStmt P C) : List P.Ident :=
+  match s with
+  | .cmd c => HasVarsImp.modifiedVars c
+  | .seq s1 s2 => KleeneStmt.modifiedVars s1 ++ KleeneStmt.modifiedVars s2
+  | .choice s1 s2 => KleeneStmt.modifiedVars s1 ++ KleeneStmt.modifiedVars s2
+  | .loop s => KleeneStmt.modifiedVars s
+
+def KleeneStmts.modifiedVars [HasVarsImp P C] (ss : List (KleeneStmt P C)) : List P.Ident :=
+  match ss with
+  | [] => []
+  | s :: srest => KleeneStmt.modifiedVars s ++ KleeneStmts.modifiedVars srest
+end
+
+instance (P : PureExpr) [HasVarsImp P C] : HasVarsImp P (KleeneStmt P C) where
+  definedVars := KleeneStmt.definedVars
+  modifiedVars := KleeneStmt.modifiedVars
+
+---------------------------------------------------------------------
+
+/-! ## Formatting -/
+
+open Std (ToFormat Format format)
+
+def formatKleeneStmt (P : PureExpr) (s : KleeneStmt P C)
+  [ToFormat P.Ident] [ToFormat P.Expr] [ToFormat P.Ty] [ToFormat C]: Format :=
+  match s with
+  | .cmd cmd => format cmd
+  | .seq s1 s2 => f!"({formatKleeneStmt P s1}) ; ({formatKleeneStmt P s2})"
+  | .choice s1 s2 => f!"({formatKleeneStmt P s1}) | ({formatKleeneStmt P s2})"
+  | .loop s => f!"({formatKleeneStmt P s})*"
+
+instance [ToFormat P.Ident] [ToFormat P.Expr] [ToFormat P.Ty] [ToFormat C]
+        : ToFormat (KleeneStmt P C) where
+  format s := formatKleeneStmt P s
+
+---------------------------------------------------------------------
+
+end -- public section
+end Imperative
